ctrl/run_on_fpga.py
@@ -6,6 +6,7 @@ from datetime import datetime
 import os
 import signal
 import sys
+import json
 
 # Workaround for pynq overriding the default SIGINT handler for some reason
 # (Hopefully no cleanup is done in custom handler?)
@@ -58,45 +59,51 @@ def _get_uio_device(irq):
     return None
 
 
-# Super inefficient, should use string buffer instead
-def print_interrupt_msg(mem):
-    num = min(mem[0] & 0xFF, 63)
+def tokenize(s):
+    return filter(lambda s: s, s.split(' '))
 
-    for addr in range(0, 16):
-        val = mem[addr]
 
-        for i in range(4):
-            # First byte is the length...
-            if addr == 0 and i == 0:
-                continue
+def word_of_bytes(bs):
+    return bs[0] | (bs[1] << 8) | (bs[2] << 2*8) | (bs[3] << 3*8)
 
-            # Max number of chars reached?
-            bytenum = 4*addr + i
 
-            if bytenum > num:
-                print()
-                return
+def words_of_bytes(bs):
+    lenbs = len(bs)
 
-            # If not, print current char
-            c = 0xFF & (val >> 8*i)
-            print(chr(c), end='')
+    if lenbs >= 4:
+        return [word_of_bytes(bs[:4])] + words_of_bytes(bs[4:])
+    elif lenbs == 3:
+        return [bs[0] | (bs[1] << 8) | (bs[2] << 2*8)]
+    elif lenbs == 2:
+        return [bs[0] | (bs[1] << 8)]
+    elif lenbs == 1:
+        return [bs[0]]
+    else:
+        return []
+
+
+def flatten(l):
+    return sum(l, [])
+
+
+def print_debug_char(c):
+    print(c, chr(c))
 
 
 def main():
     parser = argparse.ArgumentParser()
     parser.add_argument("--debug", action="store_true")
+    parser.add_argument("--args", help="Argv arguments, note that separate arguments must be separates by spaces only")
+    parser.add_argument("--stdin", help="Contents to preload stdin buffer with")
 
     parser.add_argument("bit_file", metavar="bit-file",
                         help="FPGA bitstream to load onto the FPGA")
-    parser.add_argument("--low_mem_padding", type=int, default=0)
 
-    parser.add_argument('mems', nargs='+')
+    parser.add_argument('program')
     args = parser.parse_args()
 
-    # Sanity check params
-    if len(args.mems) > 2:
-        log("Too many mem params!")
-        sys.exit(1)
+    with open(args.program) as f:
+        jsonprg = json.load(f)
 
     # Interrupt handling
     idev_file = _get_uio_device(61)
@@ -112,36 +119,97 @@ def main():
         mem_start = mem.physical_address
         log("Memory starts at", format(mem_start, '0x'))
 
-        # 4-alignment required by CakeML, redundant, but just to be clear
+        # 4-alignment required by CakeML
         if mem_start % 4 != 0:
             log("Memory start not 4-aligned, exiting")
             sys.exit(1)
 
-        # 64-alignment required by processor caches
+        # 64-alignment required by processor caches (currently disabled),
+        # redundant, but just to be clear
         if mem_start % 64 != 0:
             log("Memory start not 64-aligned, exiting")
             sys.exit(1)
 
-        # Load program from file
-        log("Loading low mem at physical addr mem_start")
-        low_mem_size = 0
-        with open(args.mems[0]) as f:
-            for i, val in enumerate(f):
-                mem[args.low_mem_padding + i] = int(val, 16)
-                #print("--> Wrote ", to_hex(int(val, 16)), "to addr", args.low_mem_padding + i)
-                low_mem_size = i
+        # Load startup code
+        log("Loading startup code at physical addr mem_start")
+        for i, val in enumerate(jsonprg["startup_code"]):
+            mem[i] = val
+            #print("--> Wrote ", to_hex(int(val, 16)), "to addr", args.low_mem_padding + i)
 
-        if len(args.mems) == 2:
-            # TODO: This value should not be hard-coded,
-            # and should be read from some memory input format instead
-            heap_block = 31457239
-            high_mem_start = (low_mem_size + 1) + heap_block
-            log("Loading high mem at physical addr",
-                format(high_mem_start + mem_start, '0x'))
+        # Pointer to where to write next in memory...
+        mempointer = len(jsonprg["startup_code"])
 
-            with open(args.mems[1]) as f:
-                for i, val in enumerate(f):
-                    mem[high_mem_start + i] = int(val, 16)
+        # Write cline
+        log("Cline...")
+
+        cline_args_size = jsonprg["cline_args_size"]
+
+        if args.args is None:
+            mempointer += 1 + cline_args_size
+        else:
+            cakeml_args = tokenize(args.args)
+
+            # cline arg count
+            mem[mempointer] = len(cakeml_args)
+            mempointer += 1
+
+            # cline args
+            cakeml_args = flatten(map(lambda arg: map(ord, arg) + [0], cakeml_args))
+
+            if len(cakeml_args) >= 4*cline_args_size:
+                log("Too long program arguments")
+                sys.exit(1)
+
+            if not all(map(allowed_char, cakeml_args)):
+                log('Program arguments contain illegal chars')
+                sys.exit(1)
+
+            for i, w in enumerate(words_of_bytes(cakeml_args)):
+                mem[mempointer + i] = w
+
+            mempointer += cline_args_size
+
+        # stdin
+
+        # stdin pointer
+        mempointer += 1
+
+        if args.stdin is None:
+            stdin = bytes()
+        else:
+            with open(args.stdin, 'rb') as f:
+                stdin = f.read()
+
+        # stdin length
+        mem[mempointer] = len(stdin)
+        mempointer += 1
+
+        # stdin
+        for i, w in enumerate(words_of_bytes(stdin)):
+            mem[mempointer + i] = w
+
+        mempointer += jsonprg["stdin_size"]
+
+        start_of_stdin = mempointer
+
+        # stderr + stdout not written from python script...
+
+        mempointer += jsonprg["output_buffer_size"]
+
+        # ffi code
+
+        for i, w in enumerate(jsonprg["ffi_code"]):
+            mem[mempointer + i] = w
+
+        mempointer += len(jsonprg["ffi_code"])
+
+        # skip stack/heap as well
+
+        mempointer += jsonprg["heap_and_stack_size"]
+
+        # ffi call jumps + cakeml data + code
+        for i, w in enumerate(jsonprg["top_mem"]):
+            mem[mempointer + i] = w
 
         # Setup FPGA
         ol = Overlay(args.bit_file)
@@ -160,7 +228,14 @@ def main():
 
             log("Got interrupt", interrupt_num, "!")
 
-            print_interrupt_msg(mem)
+            #print_interrupt_msg(mem, start_of_stdin)
+            for i in range(0, 10):
+                w = mem[start_of_stdin + i]
+
+                print_debug_char(w & 0xFF)
+                print_debug_char((w >> 8*1) & 0xFF)
+                print_debug_char((w >> 8*2) & 0xFF)
+                print_debug_char((w >> 8*3) & 0xFF)
 
             # Respond to interrupt
             core_ctrl.write(_CORE_CTRL_REG_INTERRUPT_ACK, 0)
